base soundness on lifting

Superposition_Calculus/First_Order_Superposition.thy
@@ -193,7 +193,7 @@ next
     using superposition_if_neg_superposition superposition_if_pos_superposition by metis
 qed
 
-(* TODO: Move these? *)
+(* TODO: Move these? 
 abbreviation true_clause :: 
   "'f ground_atom interp \<Rightarrow> ('f, 'v) atom clause \<Rightarrow> bool" (infix "\<TTurnstile>\<^sub>C" 50)  where
   "I \<TTurnstile>\<^sub>C C \<equiv> \<forall>\<theta>. term_subst.is_ground_subst \<theta> \<longrightarrow> I \<TTurnstile> to_ground_clause (C \<cdot> \<theta>)"
@@ -208,7 +208,7 @@ definition entails\<^sub>F ::
   "entails\<^sub>F N\<^sub>1 N\<^sub>2 \<longleftrightarrow> (\<forall>(I :: 'f gterm rel).
     refl I \<longrightarrow> trans I \<longrightarrow> sym I \<longrightarrow> compatible_with_gctxt I \<longrightarrow>
     (\<lambda>(t\<^sub>1, t\<^sub>2). Upair t\<^sub>1 t\<^sub>2) ` I \<TTurnstile>\<^sub>C\<^sub>s N\<^sub>1 \<longrightarrow>
-    (\<lambda>(t\<^sub>1, t\<^sub>2). Upair t\<^sub>1 t\<^sub>2) ` I \<TTurnstile>\<^sub>C\<^sub>s N\<^sub>2)"
+    (\<lambda>(t\<^sub>1, t\<^sub>2). Upair t\<^sub>1 t\<^sub>2) ` I \<TTurnstile>\<^sub>C\<^sub>s N\<^sub>2)"*)
 
 end
 
