Superposition_Calculus/Grounded_First_Order_Superposition.thy
@@ -1,10 +1,13 @@
 theory Grounded_First_Order_Superposition
-  imports First_Order_Superposition
+  imports 
+    First_Order_Superposition
+    Ground_Superposition_Completeness
 begin
 
 locale grounded_first_order_superposition_calculus =
-  first_order_superposition_calculus +
-  grounded_first_order_select
+  first_order_superposition_calculus select +
+  grounded_first_order_select select
+  for select :: "('f, 'v) select"
 begin
 
 sublocale ground: ground_superposition_calculus "(\<prec>\<^sub>t\<^sub>G)" select\<^sub>G
@@ -35,7 +38,135 @@ definition inference_groundings
   \<and> ground_inference \<in> ground.G_Inf
 }"
 
+lemma inference\<^sub>G_concl_in_clause_grounding: 
+  assumes "\<iota>\<^sub>G \<in> inference_groundings \<iota>"
+  shows "concl_of \<iota>\<^sub>G \<in> clause_groundings (concl_of \<iota>)"
+proof-
+  obtain premises\<^sub>G conlcusion\<^sub>G where
+    \<iota>\<^sub>G: "\<iota>\<^sub>G = Infer premises\<^sub>G conlcusion\<^sub>G"
+    using Calculus.inference.exhaust by blast
+
+  obtain "premises" conlcusion where
+    \<iota>: "\<iota> = Infer premises conlcusion"
+    using Calculus.inference.exhaust by blast
+
+  obtain \<theta> where 
+    "is_ground_clause (conlcusion \<cdot> \<theta>)"
+    "conlcusion\<^sub>G = to_ground_clause (conlcusion \<cdot> \<theta>)"
+    using assms list_4_cases
+    unfolding inference_groundings_def \<iota> \<iota>\<^sub>G Calculus.inference.case
+    by(simp split: list.splits)(metis list_4_cases) 
+
+  then show ?thesis
+    unfolding \<iota> \<iota>\<^sub>G clause_groundings_def
+    by auto
+qed  
+
+lemma inference\<^sub>G_red_in_clause_grounding_of_concl: 
+  assumes "\<iota>\<^sub>G \<in> inference_groundings \<iota>"
+  shows "\<iota>\<^sub>G \<in> ground.Red_I (clause_groundings (concl_of \<iota>))"
+proof-
+  from assms have "\<iota>\<^sub>G \<in> ground.G_Inf"
+    unfolding inference_groundings_def
+    by blast
+
+  moreover have "concl_of \<iota>\<^sub>G \<in> clause_groundings (concl_of \<iota>)"
+    using assms inference\<^sub>G_concl_in_clause_grounding
+    by auto
+
+  ultimately show "\<iota>\<^sub>G \<in> ground.Red_I (clause_groundings (concl_of \<iota>))"
+    using ground.Red_I_of_Inf_to_N
+    by blast
+qed
+
 end
+
+(* TODO: some *)
+sublocale first_order_superposition_calculus \<subseteq>
+  lifting_intersection
+    inferences      
+    "{{#}}"
+    select\<^sub>G\<^sub>s
+    "ground_superposition_calculus.G_Inf (\<prec>\<^sub>t\<^sub>G)"               
+    "\<lambda>_. ground_superposition_calculus.G_entails" 
+    "ground_superposition_calculus.GRed_I (\<prec>\<^sub>t\<^sub>G)" 
+    "\<lambda>_. ground_superposition_calculus.GRed_F(\<prec>\<^sub>t\<^sub>G)" 
+    "\<bottom>\<^sub>F"
+    "\<lambda>_. clause_groundings" 
+    "\<lambda>select\<^sub>G.  Some \<circ> (grounded_first_order_superposition_calculus.inference_groundings (\<prec>\<^sub>t) select\<^sub>G)"
+    tiebreakers
+proof(unfold_locales; (intro ballI)?)
+  show "select\<^sub>G\<^sub>s \<noteq> {}"
+    using select\<^sub>G_simple
+    unfolding select\<^sub>G\<^sub>s_def 
+    by blast
+next 
+  fix select\<^sub>G
+  assume "select\<^sub>G \<in> select\<^sub>G\<^sub>s"
+ 
+  then interpret grounded_first_order_superposition_calculus _ _ select\<^sub>G
+    apply unfold_locales
+    by(simp add: select\<^sub>G\<^sub>s_def)
+
+  show "consequence_relation ground.G_Bot ground.G_entails"
+    using ground.consequence_relation_axioms.
+next
+   fix select\<^sub>G
+   assume "select\<^sub>G \<in> select\<^sub>G\<^sub>s"
+ 
+  then interpret grounded_first_order_superposition_calculus _ _ select\<^sub>G
+    apply unfold_locales
+    by(simp add: select\<^sub>G\<^sub>s_def)
+
+  show "tiebreaker_lifting
+          \<bottom>\<^sub>F
+          inferences 
+          ground.G_Bot
+          ground.G_entails
+          ground.G_Inf 
+          ground.GRed_I
+          ground.GRed_F 
+          clause_groundings
+          (Some \<circ> inference_groundings)
+          tiebreakers"
+  proof unfold_locales
+    show "\<bottom>\<^sub>F \<noteq> {}"
+      by simp
+  next
+    fix bottom
+    assume "bottom \<in> \<bottom>\<^sub>F"
+
+    then show "clause_groundings bottom \<noteq> {}"
+      unfolding clause_groundings_def 
+      by simp
+  next
+    fix bottom
+    assume "bottom \<in> \<bottom>\<^sub>F"
+    then show "clause_groundings bottom \<subseteq> ground.G_Bot"
+      unfolding clause_groundings_def
+      by simp
+  next
+    fix clause
+    show "clause_groundings clause \<inter> ground.G_Bot \<noteq> {} \<longrightarrow> clause \<in> \<bottom>\<^sub>F"
+      unfolding clause_groundings_def to_ground_clause_def subst_clause_def
+      by simp
+  next
+    fix \<iota>   
+    show "the ((Some \<circ> inference_groundings) \<iota>) 
+                \<subseteq> ground.GRed_I (clause_groundings (concl_of \<iota>))"
+      using inference\<^sub>G_red_in_clause_grounding_of_concl
+      by auto
+  next
+    show "\<And>g. po_on (tiebreakers g) UNIV"
+      unfolding po_on_def
+      using wellfounded_tiebreakers
+      by simp
+  next
+    show "\<And>g. wfp_on (tiebreakers g) UNIV"
+      using wellfounded_tiebreakers
+      by simp
+  qed
+qed
 
 end
 
